\begin{enumerate}[a)]
  \item Soit $g,h\in C_G(S)$. Pour tout $x\in S$, on a
    \[
      (gh^{-1})x(gh^{-1})^{-1} = (gh^{-1})x(hg^{-1})
      = g(h^{-1}xh)g^{-1}
      = gxg^{-1} \\
      = x.
    \]
    Donc $gh^{-1}\in C_G(S)$ et $C_G(S)$ est un sous-groupe de $G$.

  \item $g\in Z(G) \Leftrightarrow \forall x\in G,\: gx=xg
    \Leftrightarrow \forall x\in G,\: g\in C_G(x)
    \Leftrightarrow g\in\cap_{x\in G} C_G(x)$.
  
  \item $H = C_G(x) \Leftrightarrow \forall h\in H,\: hx=xh 
    \Leftrightarrow x\in Z(H)$.
\end{enumerate}

