Posons $\gamma' = (j_1,j_r)(j_1,j_{r-1})\dots (j_1,j_2)$.
Si $j\in\N_n\setminus\set{j_1,j_2,\dots,j_r}$, alors $\gamma'(k) = k = \gamma(k)$.
Si $k\in\N_{r-1}$, alors
%
\begin{align*}
  \gamma'(j_k)
    &= (j_1,j_r)\dots (j_1,j_2) (j_k) \\
    &= (j_1,j_r)\dots(j_1,j_k)(j_k) \\
    &= \dots(j_1,j_{k+1})(j_1) \\
    &= j_{k+1} \\
    &= \gamma(j_k).
\end{align*}
%
Et enfin $\gamma'(j_r) = (j_1,j_r)(j_r) = j_1 = \gamma(j_r)$.
Par conséquent $\gamma' = \gamma$, c'est-à-dire
\[
  (j_1,j_2,\dots,j_r) = (j_1,j_r)(j_1,j_{r-1})\dots (j_1,j_2).
\]
